Experiment

src/specs/EvaluateLagrangePolyOutOfDomain.ec
@@ -67,8 +67,8 @@ module EvaluateLagrangePolyOutOfDomain = {
   proc mid(polyNum: int, at: int): int option = {
     var r, omegaPolyNum, atDomainSize, zd1, num, den, inv;
 
-    omegaPolyNum <- (OMEGA ^ polyNum) %% R; (* Modexp.mid(..., ...) *)
-    atDomainSize <- (at ^ DOMAIN_SIZE) %% R; 
+    omegaPolyNum <@ Modexp.mid(OMEGA,polyNum);
+    atDomainSize <@ Modexp.mid(at, DOMAIN_SIZE); 
     zd1 <- (atDomainSize - 1) %% R;
     
     if(zd1 = 0) { (* (at ^ DOMAIN_SIZE) - 1 = 0 *)
@@ -76,7 +76,7 @@ module EvaluateLagrangePolyOutOfDomain = {
     } else {
       num <- (omegaPolyNum * zd1) %% R;
       den <- (DOMAIN_SIZE * (at - omegaPolyNum)) %% R;
-      inv <- den^(R - 2) %% R;
+      inv <@ Modexp.mid(den, R - 2);
       r <- Some ((num * inv) %% R);
       (* ((OMEGA ^ polyNum) * (atDomainSize - 1))
         ----------------------------------------
@@ -128,16 +128,31 @@ lemma modexp_same (m: mem) (v1 v2 p1 p2 r1 r2 : uint256) :
     modexp_memory_footprint m v2 p2 r2.
 proof. admit. qed.
 
-lemma modexp_pspec (m : mem) (base power : uint256) :
-    phoare [ Modexp.low :
-      arg = (base, power) /\
-      Primops.memory = m /\
-      !Primops.reverted
+(* lemma modexp_pspec (m : mem) (base power : uint256) : *)
+(*     phoare [ Modexp.low : *)
+(*       arg = (base, power) /\ *)
+(*       Primops.memory = m /\ *)
+(*       !Primops.reverted *)
+(*       ==> *)
+(*       !Primops.reverted /\ *)
+(*       Primops.memory = modexp_memory_footprint m base power res /\ *)
+(*       res = W256.of_int (((W256.to_uint base) ^ (W256.to_uint power)) %% R) *)
+(*     ] = 1%r. *)
+(* proof. admit. qed. *)
+
+lemma modexp_low_equiv_mid_test (memory: mem) (value256 power256: uint256):
+    equiv [
+      Modexp.low ~ Modexp.mid:
+      arg{1} = (value256, power256) /\
+      arg{2} = (W256.to_uint value256, W256.to_uint power256) /\
+      !Primops.reverted{1} /\
+      Primops.memory{1} = memory    
       ==>
-      !Primops.reverted /\
-      Primops.memory = modexp_memory_footprint m base power res /\
-      res = W256.of_int (((W256.to_uint base) ^ (W256.to_uint power)) %% R)
-    ] = 1%r.
+      res{2} = W256.to_uint res{1} /\
+      !Primops.reverted{1} /\
+      0 <= res{2} < R /\
+      Primops.memory{1} = (modexp_memory_footprint memory value256 power256 res{1})
+    ].
 proof. admit. qed.
 
 lemma modexp_low_pspec_revert :
@@ -152,16 +167,9 @@ equiv [
       !Primops.reverted{1} /\
       Primops.memory{1} = memory
       ==>
-      (
-        !Primops.reverted{1} /\
-        ((W256.to_uint at256)^DOMAIN_SIZE - 1) %% Constants.R <> 0 /\
-        res{2} = Some (to_uint res{1})%W256)
+      (!Primops.reverted{1} /\ res{2} = Some (to_uint res{1})%W256)
       \/
-      (
-        Primops.reverted{1} /\
-        ((W256.to_uint at256)^DOMAIN_SIZE - 1) %% Constants.R = 0 /\
-        res{2} = None
-      )
+      (Primops.reverted{1} /\ res{2} = None)
     ].
 proof. proc.
     
@@ -170,126 +178,114 @@ seq 2 1 : (
   (polyNum{2}, at{2}) = (to_uint poly256, to_uint at256) /\
   !Primops.reverted{1} /\
   ((poly256 <> W256.zero /\ Primops.memory{1} = (modexp_memory_footprint memory (W256.of_int OMEGA) polyNum{1} omegaPower{1})) 
-  \/
-  (poly256 = W256.zero /\ Primops.memory{1} = memory)
-  )
+    \/
+  (poly256 = W256.zero /\ Primops.memory{1} = memory))
   /\
-  omegaPower{1} = W256.of_int omegaPolyNum{2} /\ omegaPolyNum{2} = (OMEGA ^ polyNum{2}) %% R
-). wp. sp. 
+  omegaPower{1} = W256.of_int omegaPolyNum{2} /\ 0 <= omegaPolyNum{2} < R
+). sp. 
 case (bool_of_uint256 polyNum{1}).
 (* polyNum != 0 *)
 rcondt{1} 1. by progress.
-call{1} (modexp_pspec memory (W256.of_int OMEGA) poly256).
-skip. progress. left. by auto.
-rewrite !W256.of_uintK. have ->: OMEGA %% W256.modulus = OMEGA. by smt(). by reflexivity.
+call (modexp_low_equiv_mid_test memory (W256.of_int OMEGA) poly256).
+(* call{1} (modexp_pspec memory (W256.of_int OMEGA) poly256). *)
+skip. progress. by smt. left. by auto.
 rcondf{1} 1. by progress.
-skip. progress. right. by auto.
-have ->: polyNum{1} = W256.zero. by smt(). progress. by smt().
+inline Modexp.mid. wp. skip. progress. right. by auto.
+have ->: polyNum{1} = W256.zero. by auto. by smt().
+have ->: polyNum{1} = W256.zero. by auto. by smt().
+have ->: polyNum{1} = W256.zero. by auto. by smt().
 
 seq 1 1: (
   (polyNum{1}, at{1}) = (poly256, at256) /\
   (polyNum{2}, at{2}) = (to_uint poly256, to_uint at256) /\
   !Primops.reverted{1} /\
   Primops.memory{1} = modexp_memory_footprint memory at{1} (W256.of_int DOMAIN_SIZE) tmp267{1} /\
-  omegaPower{1} = W256.of_int omegaPolyNum{2} /\ omegaPolyNum{2} = (OMEGA ^ polyNum{2}) %% R /\
-  tmp267{1} = W256.of_int atDomainSize{2} /\ atDomainSize{2} = (at{2} ^ DOMAIN_SIZE) %% R
+  omegaPower{1} = W256.of_int omegaPolyNum{2} /\ 0 <= omegaPolyNum{2} < R /\
+  tmp267{1} = W256.of_int atDomainSize{2} /\ 0 <= atDomainSize{2} < R
 ).
 wp. 
 exists* omegaPower{1}. elim* => oP.
 pose mem' := (modexp_memory_footprint memory ((of_int OMEGA))%W256 poly256 oP).
 case (poly256 = W256.zero).
-call{1} (modexp_pspec memory at256 (W256.of_int DOMAIN_SIZE)).
-skip. progress. by smt().
-rewrite !W256.of_uintK. have ->: DOMAIN_SIZE %% W256.modulus = DOMAIN_SIZE. by smt(). reflexivity.
-call{1} (modexp_pspec mem' at256 (W256.of_int DOMAIN_SIZE)).
-skip. progress. by smt(). apply modexp_same.
-rewrite !W256.of_uintK. have ->: DOMAIN_SIZE %% W256.modulus = DOMAIN_SIZE. by smt(). reflexivity.
+call{1} (modexp_low_equiv_mid_test memory at256 (W256.of_int DOMAIN_SIZE)).
+skip. progress. by smt. by smt().
+call{1} (modexp_low_equiv_mid_test mem' at256 (W256.of_int DOMAIN_SIZE)).
+skip. progress. by smt. by smt(). apply modexp_same.
 
-seq 1 1: (#pre /\ ret{1} = W256.of_int zd1{2} /\ zd1{2} = (atDomainSize{2} - 1) %% R).
+seq 1 1: (#pre /\ ret{1} = W256.of_int zd1{2} /\ 0 <= zd1{2} < R).
 wp. skip. progress.
-rewrite /addmod. progress. rewrite !W256.of_uintK !mod_R_W256_mod_R !R_mod_W256_R.
-have ->: (R - 1) %% W256.modulus = R - 1. by smt(). by smt.
+rewrite /addmod. progress. rewrite !W256.of_uintK !R_mod_W256_R.
+have ->: (R - 1) %% W256.modulus = R - 1. by smt().
+have ->: atDomainSize{2} %% W256.modulus = atDomainSize{2}. by smt().
+by smt(). by smt(). by smt().
 
-if. progress.
-rewrite /bool_of_uint256 /iszero in H0.
-case ((of_int ((to_uint at{1} ^ DOMAIN_SIZE %% R - 1) %% R))%W256 = W256.zero).
-progress. by smt.
-progress. by smt.
-by smt.
+if. progress. by smt. by smt.
 
-seq 1 1: ((to_uint at256 ^ DOMAIN_SIZE - 1) %% R = 0 /\ r{2} = None /\ Primops.reverted{1}).
-wp. call{1} revertWithMessage_low_pspec. skip. progress. by smt.
-wp. sp. call{1} modexp_low_pspec_revert. skip. progress.
+seq 1 1: (r{2} = None /\ Primops.reverted{1}).
+wp. call{1} revertWithMessage_low_pspec. skip. by progress.
+wp. sp. call{1} modexp_low_pspec_revert. skip. by progress.
 
 seq 1 1: (
 (polyNum{1}, at{1}) = (poly256, at256) /\
 (polyNum{2}, at{2}) = (to_uint poly256, to_uint at256) /\
 !Primops.reverted{1} /\
 Primops.memory{1} = modexp_memory_footprint memory at{1} ((of_int DOMAIN_SIZE))%W256 tmp267{1} /\
-omegaPower{1} = (of_int omegaPolyNum{2})%W256 /\ omegaPolyNum{2} = OMEGA ^ polyNum{2} %% R /\
-tmp267{1} = (of_int atDomainSize{2})%W256 /\ atDomainSize{2} = at{2} ^ DOMAIN_SIZE %% R /\
-ret{1} = (of_int num{2})%W256 /\ num{2} = (omegaPolyNum{2} * zd1{2}) %% R /\
-zd1{2} = (atDomainSize{2} - 1) %% R /\ zd1{2} <> 0
+omegaPower{1} = (of_int omegaPolyNum{2})%W256 /\ 0 <= omegaPolyNum{2} < R /\
+tmp267{1} = (of_int atDomainSize{2})%W256 /\ 0 <= atDomainSize{2} < R /\ 0 <= zd1{2} < R /\
+ret{1} = (of_int num{2})%W256 /\ 0 <= num{2} < R
 ).
 wp. skip. progress.
-rewrite /mulmod. progress. rewrite !W256.of_uintK !mod_R_W256_mod_R !R_mod_W256_R. by smt().
-rewrite /bool_of_uint256 /iszero in H0. by smt.
+rewrite /mulmod. progress. rewrite !W256.of_uintK !R_mod_W256_R.
+have ->: zd1{2} %% W256.modulus = zd1{2}. by smt().
+have ->: omegaPolyNum{2} %% W256.modulus = omegaPolyNum{2}. by smt().
+by smt(). by smt(). by smt().
 
 seq 3 1: (
-#pre /\ denominator{1} = W256.of_int den{2} /\
-den{2} = (DOMAIN_SIZE * (at{2} - omegaPolyNum{2})) %% R
+#pre /\ denominator{1} = W256.of_int den{2} /\ 0 <= den{2} < R
 ).
 wp. skip. progress. 
 rewrite /addmod /mulmod. progress. rewrite !W256.of_uintK !R_mod_W256_R.
 have ->: DOMAIN_SIZE %% W256.modulus = DOMAIN_SIZE. by smt().
-have ->: (R - OMEGA ^ to_uint polyNum{1} %% R) %% W256.modulus = (R - OMEGA ^ to_uint polyNum{1} %% R). by smt().
-have ->: (to_uint at{1} + (R - OMEGA ^ to_uint polyNum{1} %% R)) %% R %% W256.modulus = (to_uint at{1} + (R - OMEGA ^ to_uint polyNum{1} %% R)) %% R. by smt().
-by smt().
+have ->: (R - omegaPolyNum{2}) %% W256.modulus = (R - omegaPolyNum{2}). by smt().
+rewrite !mod_R_W256_mod_R. by smt. by smt(). by smt().
 
 seq 1 1: (
 (polyNum{1}, at{1}) = (poly256, at256) /\
 (polyNum{2}, at{2}) = (to_uint poly256, to_uint at256) /\
 !Primops.reverted{1} /\
 omegaPower{1} = (of_int omegaPolyNum{2})%W256 /\
-omegaPolyNum{2} = OMEGA ^ polyNum{2} %% R /\
+0 <= omegaPolyNum{2} < R /\
 tmp267{1} = (of_int atDomainSize{2})%W256 /\
-atDomainSize{2} = at{2} ^ DOMAIN_SIZE %% R /\
+0 <= atDomainSize{2} < R /\
 ret{1} = (of_int num{2})%W256 /\
-num{2} = omegaPolyNum{2} * zd1{2} %% R /\
-zd1{2} = (atDomainSize{2} - 1) %% R /\ zd1{2} <> 0 /\
-den{2} = DOMAIN_SIZE * (at{2} - omegaPolyNum{2}) %% R /\
+0 <= num{2} < R /\
+0 <= zd1{2} < R /\
+0 <= den{2} < R /\
 Primops.memory{1} = modexp_memory_footprint memory (of_int den{2})%W256 (W256.of_int (R - 2)) denominator{1} /\
-denominator{1} = W256.of_int inv{2} /\ inv{2} = (den{2} ^ (R - 2)) %% R
+denominator{1} = W256.of_int inv{2} /\ 0 <= inv{2} < R
 ).
-sp.
+
 exists* tmp267{1}. elim* => tmp. exists* denominator{1}. elim* => d.
 pose mem' := modexp_memory_footprint memory at256 ((of_int DOMAIN_SIZE))%W256 tmp.
-call{1} (modexp_pspec mem' d ((W256.of_int R) - (W256.of_int 2))). 
-skip. progress. rewrite /mem'. apply modexp_same.
-rewrite !W256.of_uintK !mod_R_W256_mod_R.
-have ->: (R - 2) %% W256.modulus = R - 2. by smt(). by reflexivity.
-
-seq 1 1: (
-(polyNum{1}, at{1}) = (poly256, at256) /\
-(polyNum{2}, at{2}) = (to_uint poly256, to_uint at256) /\
-!Primops.reverted{1} /\
-omegaPower{1} = (of_int omegaPolyNum{2})%W256 /\
-omegaPolyNum{2} = OMEGA ^ polyNum{2} %% R /\
-tmp267{1} = (of_int atDomainSize{2})%W256 /\
-atDomainSize{2} = at{2} ^ DOMAIN_SIZE %% R /\
-(* ret{1} = (of_int num{2})%W256 /\ *)
-num{2} = omegaPolyNum{2} * zd1{2} %% R /\
-zd1{2} = (atDomainSize{2} - 1) %% R /\ zd1{2} <> 0 /\
-den{2} = DOMAIN_SIZE * (at{2} - omegaPolyNum{2}) %% R /\
-Primops.memory{1} = modexp_memory_footprint memory (of_int den{2})%W256 (W256.of_int (R - 2)) denominator{1} /\
-denominator{1} = W256.of_int inv{2} /\ inv{2} = (den{2} ^ (R - 2)) %% R /\
-ret{1} = (of_int ((num{2} * inv{2}) %% R))%W256 /\ r{2} = Some ((num{2} * inv{2}) %% R)
-).
-wp. skip. progress. 
-rewrite /mulmod. progress. 
-rewrite !W256.of_uintK !mod_R_W256_mod_R !R_mod_W256_R. by reflexivity.
-skip. progress.
-by smt().
-by smt.
+call{1} (modexp_low_equiv_mid_test mem' d ((W256.of_int R) - (W256.of_int 2))).
+skip. progress. rewrite /mem'. by smt. by smt. apply modexp_same.
+wp. skip. progress. rewrite /mulmod. progress. rewrite !W256.of_uintK !R_mod_W256_R.
+have ->: num{2} %% W256.modulus = num{2}. by smt().
+have ->: inv{2} %% W256.modulus = inv{2}. by smt().
+rewrite mod_R_W256_mod_R. by reflexivity.
 qed.
 
+lemma lagrange_pspec_mid (polyNum at: int) :
+    phoare [ EvaluateLagrangePolyOutOfDomain.mid :
+      arg = (polyNum, at)
+      ==>
+      let opR = OMEGA ^ polyNum %% R in
+      let aDR = (at ^ DOMAIN_SIZE %% R - 1) %% R in
+      let inv = (DOMAIN_SIZE * (at - opR) %% R) ^ (R - 2) %% R in
+      ((at^DOMAIN_SIZE - 1) %% Constants.R <> 0 /\ res = Some ((opR * aDR) * inv %% R))
+        \/
+      ((at^DOMAIN_SIZE - 1) %% Constants.R = 0 /\ res = None)
+    ] = 1%r.
+proof. proc.
+inline Modexp.mid; wp; skip. progress; by smt(). 
+qed.
